src/later.v
@@ -9,40 +9,78 @@ From ITree Require Import ITree.
 Variant laterE : Type → Type :=
   | ELater : laterE ().
 
+Definition step `{laterE -< E} : itree E () :=
+  trigger ELater.
+
 Global Instance AnswerEqDecision_laterE :
   AnswerEqDecision laterE.
 Proof. intros A [] [] []. by left. Qed.
 
+Variant later_modality : Set :=
+  | Identity
+  | Later.
+
+Definition lat {Σ} (m : later_modality) (P : iProp Σ) : iProp Σ :=
+  match m with
+  | Identity => P
+  | Later => ▷ P
+  end.
+
+Section lat.
+  Lemma lat_mono {Σ} m (Φ Ψ : iProp Σ) :
+    (Φ -∗ Ψ) -∗
+    lat m Φ -∗ lat m Ψ.
+  Proof.
+    iIntros "Hwand HΦ". destruct m; by iApply "Hwand".
+  Qed.
+
+  Lemma lat_intro {Σ} m (Φ : iProp Σ) :
+    Φ -∗
+    lat m Φ.
+  Proof.
+    iIntros "HΦ". by destruct m.
+  Qed.
+
+  Lemma lat_sep {Σ} m (Φ Ψ : iProp Σ) :
+    lat m Φ -∗
+    lat m Ψ -∗
+    lat m (Φ ∗ Ψ).
+  Proof.
+    iIntros "HΦ HΨ". destruct m; iFrame.
+  Qed.
+End lat.
+
 Section handler.
   Context {Σ : gFunctors}.
 
-  Program Definition laterH : iHandler Σ laterE :=
+  Program Definition laterH (m : later_modality) : iHandler Σ laterE :=
     IHandler (λ A e,
       match e with
-      | ELater => λ Φ _, ▷ Φ ()
+      | ELater => λ Φ _, lat m (Φ ())
       end
     )%I _.
   Next Obligation.
-    iIntros (??????) "HΦwand _". destruct e.
-    iIntros "HΦ". iNext. by iApply "HΦwand".
+    iIntros (???????) "HΦwand _". destruct e.
+    iIntros "HΦ". by iApply (lat_mono with "HΦwand").
   Qed.
-  Global Instance laterH_Sequential :
-    Sequential laterH.
+  Global Instance laterH_Sequential m :
+    Sequential (laterH m).
   Proof.
     by iIntros (A [] Φ s) "HH".
   Qed.
 End handler.
 
 Section wpi_later.
-  Context `{!invGS_gen hlc Σ} {E : Type → Type} {H : iHandler Σ E}.
-  Context `{laterE -< E} `{inH Σ laterE E laterH H}.
+  Context `{!invGS_gen hlc Σ} {E : Type → Type} {H : iHandler Σ E} {m : later_modality}.
+  Context `{laterE -< E} `{inH Σ laterE E (laterH m) H}.
 
   Lemma wpi_later M (Φ : () → iProp Σ) :
-    (▷ |={M}=> Φ ()) -∗
+    (lat m (|={M}=> Φ ())) -∗
     WPi (trigger ELater) @ H; M {{ Φ }}.
   Proof.
     iIntros "HΦ". iApply wpi_vis.
     iApply fupd_mask_intro; first apply empty_subseteq. iIntros "Hfupd".
-    iApply is_inH. simpl. iNext. iApply wpi_ret. by iMod "Hfupd".
+    iApply is_inH. simpl. iApply (lat_mono with "[Hfupd]"); last done.
+    iIntros "HΦ". iApply wpi_ret. by iMod "Hfupd".
   Qed.
 End wpi_later.
